\documentclass[10pt]{article}
\usepackage{graphicx}
\usepackage{amssymb}
\usepackage[fleqn]{amsmath}
\usepackage{nccmath}
\usepackage{cases}
\usepackage{hyperref}
\usepackage{multicol}
\usepackage{tikz}
\usepackage{tikz}
\usetikzlibrary{shapes.geometric}
\usepackage{pgfplots}
\usepackage{enumitem}
\pgfplotsset{compat=1.18}
\usepackage{float}

\title{\bf Math 106: Problem Set 6}
\date{2/25/2024}
\author{\bf Owen Jones}
\begin{document}
\begin{enumerate}
    \item [\textbf{7.2.1}] Let $x=x'\cos\theta-y'\sin\theta$ and $y=x'\sin\theta+y'\cos\theta$.
    \begin{align*}
        &ax^2=a{x'}^2\cos^2\theta-ax'y'\sin2\theta+a{y'}^2\sin^2\theta\\
        &bxy=b{x'}^2\sin\theta\cos\theta+bx'y'\cos2\theta-b{y'}^2\sin\theta\cos\theta\\
        &cy^2=c{x'}^2\sin^2\theta+cx'y'\sin2\theta+c{y'}^2\cos^2\theta
    \end{align*}
    Collecting like terms
    \begin{align*}
        &(a\cos^2\theta+b\sin\theta\cos\theta+c\sin^2\theta){x'}^2=(a+\frac{b}{2}\sin2\theta+(c-a)\frac{1-\cos2\theta}{2}){x'}^2\\
        &((c-a)'\sin2\theta+b\cos2\theta)x'y'={x'}^2{y'}^2\\
        &(a\sin^2\theta-b\sin\theta\cos\theta+c\cos^2\theta){y'}^2=(a-\frac{b}{2}\sin2\theta+(c-a)\frac{1+\cos2\theta}{2}){y'}^2
    \end{align*}
        We want to choose a suitable $\theta$ s.t $x'y'=0$. Let $\theta^*=\frac{\arctan(\frac{a-c}{b})}{2}$

        Let $a'=a+\frac{b}{2}\sin2\theta^*+(c-a)\frac{1-\cos2\theta^*}{2}$ and $b'=a-\frac{b}{2}\sin2\theta^*+(c-a)\frac{1+\cos2\theta^*}{2}$.\\
       This gives us the desired form $a'{x'}^2+b'{y'}^2$
    \item [\textbf{7.2.2}] Let $f(x,y)=ax^2+bxy+cy^2+dx+ey+f$ be some quadratic function.\\
    \textbf{7.2.1} allows us to simplify $ax^2+bxy+cy^2\rightarrow a'{x'}^2+b'{y'}^2$.
    Applying the substitution from \textbf{7.2.1}
    $dx+ey+f=d(x'\cos\theta-y'\sin\theta)+e(x'\sin\theta+y'\cos\theta)+f=(d\cos\theta+e\sin\theta)x'+(e\cos\theta-d\sin\theta)y'+f$\\
    Thus, any quadratic can be expressed as $a'{x'}^2+b'{y'}^2+c'x'+dx'+e'$
    \item [\textbf{7.3.1}] Substituting $x=\frac{3at}{1+t^3}$ and $y=\frac{3at^2}{1+t^3}$ into $x^3+y^3=3axy$
    \begin{align*}
        &x^3+y^3\\
        &{(\frac{3at}{1+t^3})}^3+{(\frac{3at^2}{1+t^3})}^3\\
        &=\frac{27a^3t^3}{{(1+t^3)}^3}+\frac{27a^3t^6}{{(1+t^3)}^3}\\
        &=\frac{27a^3t^3(1+t^3)}{{(1+t^3)}^3}=3a\frac{9a^2t^3}{{(1+t^3)}^2}\\
        &=3a\frac{3at}{1+t^3}\frac{3at^2}{1+t^3}\\
        &=3axy
    \end{align*}
    $x=\frac{3at}{1+t^3}$ and $y=\frac{3at^2}{1+t^3}$ parameterize the folium.
    At $t=0$ $x=\frac{3a\cdot0}{1+0^3}=0$ and $y=\frac{3a\cdot 0^2}{1+0^3}=0$, so the folium lies on the $x$ and $y$ axis at $0$.
    \item [\textbf{7.3.2}] $x^3+y^3$ can be factored as $(x+y)(x^2-xy+y^2)$. It follows
    \begin{align*}
        &x^3+y^3=3axy\\
        &\Rightarrow x+y=\frac{3axy}{x^2-xy+y^2} \text{ where }(x,y)\neq(0,0)\\
        &\Rightarrow x+y=\frac{3a}{\frac{x}{y}+\frac{y}{x}-1}\frac{xy}{xy} \text{ where }x,y\neq=0\\
        &\Rightarrow x+y=\frac{3a}{\frac{x}{y}+\frac{y}{x}-1}
    \end{align*}
    \item [\textbf{7.3.3}] $t\rightarrow -1^-\Rightarrow x\rightarrow +\infty$ and $t\rightarrow -1^+\Rightarrow x\rightarrow -\infty$.\\
    $\frac{x}{y}=\frac{1}{t}$ and $\frac{y}{x}=\frac{t}{1}$, so $\frac{x}{y}\rightarrow\frac{1}{-1}=-1$ and $\frac{y}{x}\rightarrow\frac{-1}{1}=-1$
    \item [\textbf{7.4.1}] $x=t^2$ and $y^3$ is a simple parameterization by inspection. Finding the second intersection point of the line $y=tx$ we obtain:
    \begin{align*}
        &y^2=x^3\\
        &{(xt)}^2=x^3\\
        &x^2t^2=x^3\\
        &t^2x^2-x^3=0\\
        &x^2(t^2-x)
    \end{align*}
    , so our points of intersection are $x=0$ and $x=t^2$. Thus, we again choose the parameterization $x=t^2$ and $y=t^3$.
\end{enumerate}
\end{document}