\documentclass[10pt]{article}
\usepackage{graphicx}
\usepackage{amssymb}
\usepackage[fleqn]{amsmath}
\usepackage{nccmath}
\usepackage{cases}
\usepackage{hyperref}
\usepackage{multicol}
\usepackage{tikz}
\usepackage{pgfplots}
\usepackage{enumitem}
\usepackage{pdfpages}
\pgfplotsset{compat=1.18}
\usepackage{float}
\DeclareMathOperator*{\argmin}{arg\,min}

\title{\bf Math 164: Problem Set 8}
\date{3/1/2024}
\author{\bf Owen Jones}
\begin{document}
\maketitle
\begin{enumerate}
    \item [\textbf{10.10}] \begin{enumerate}
        \item $f(x)=\frac{1}{2}\mathbf{x}^\top\begin{bmatrix}
            5 & 2\\
            2 & 1
        \end{bmatrix}\mathbf{x}-\mathbf{x}^\top\begin{bmatrix}
            3\\
            1
        \end{bmatrix}$
        \item $\mathbf{d}^{(0)}=-\mathbf{g}^{(0)}=-\begin{bmatrix}
            5 & 2\\
            2 & 1
        \end{bmatrix}\mathbf{x}^{(0)}+\begin{bmatrix}
            3\\
            1
        \end{bmatrix}=\begin{bmatrix}
            3\\
            1
        \end{bmatrix}$,\\
        $\alpha_0=\frac{5}{29}$,\\ 
        $\mathbf{x}^{(1)}=\begin{bmatrix}
            \frac{15}{29}\\
            \frac{5}{29}
        \end{bmatrix}$\\
        $\mathbf{g}^{(1)}=\begin{bmatrix}
            5 & 2\\
            2 & 1
        \end{bmatrix}\begin{bmatrix}
            \frac{15}{29}\\
            \frac{5}{29}
        \end{bmatrix}-\begin{bmatrix}
            3\\
            1
        \end{bmatrix}=\begin{bmatrix}
            -\frac{2}{29}\\
            \frac{6}{29}
        \end{bmatrix}$,\\ 
        $\beta_0=\frac{{\mathbf{g}^{(1)}}^\top\mathbf{Q}\mathbf{d}^{(0)}}{{\mathbf{d}^{(0)}}^\top\mathbf{Q}\mathbf{d}^{(0)}}=\frac{4}{841}$\\
        $\mathbf{d}^{(1)}=-\mathbf{g}^{(1)}+\beta_k\mathbf{d}^{(0)}=\begin{bmatrix}
            \frac{2}{29}\\
            -\frac{6}{29}
        \end{bmatrix}+\frac{4}{841}\begin{bmatrix}
            3\\
            1
        \end{bmatrix}=\begin{bmatrix}
            \frac{70}{841}\\
            -\frac{170}{841}
        \end{bmatrix}$\\
        $\alpha_1=\frac{\frac{1160}{24389}}{\frac{5800}{841^2}}=\frac{29}{5}$\\
        $\mathbf{x}^{(2)}=\begin{bmatrix}
            \frac{15}{29}\\
            \frac{5}{29}
        \end{bmatrix}+\frac{29}{5}\begin{bmatrix}
            \frac{70}{841}\\
            -\frac{170}{841}
        \end{bmatrix}=\begin{bmatrix}
            1\\
            -1
        \end{bmatrix}$
        \item By the FONC $\mathbf{x}^*=\mathbf{Q}^{-1}\mathbf{b}=\begin{bmatrix}
            1 & -2\\
            -2 & 5
        \end{bmatrix}\begin{bmatrix}
            3\\
            1
        \end{bmatrix}=\begin{bmatrix}
            1\\
            -1
        \end{bmatrix}$ which agrees with the result from part (b).
    \end{enumerate}
    \item [\textbf{12.1}] $\underset{m}{\argmin}{\lVert \mathbf{A}m-\mathbf{F}\rVert}^2$ where $\mathbf{A}=\begin{bmatrix}
        3\\
        5\\
        6
    \end{bmatrix},\mathbf{F}\begin{bmatrix}
        1\\
        2\\
        3
    \end{bmatrix}$. $m^*={\mathbf{A}^\top\mathbf{A}}^{-1}\mathbf{A}^\top\mathbf{F}=\frac{31}{70}$
    \item [\textbf{12.8}] 
    $\displaystyle y_0=0\\
    y_1=bu_1+v_1\\
    y_2=abu_1+av_1+bu_2+v_2\\
    \ldots\\
    y_k=\sum_{i=1}^{k}a^{k-i} bu_i+a^{k-i}v_i$\\
    Let $\mathbf{C}:=\begin{bmatrix}
        b & 0 & \cdots & 0\\
        ba & b & \ddots & \vdots\\
        \vdots & \ddots & \ddots & \vdots\\
        ba^{n-1} & \cdots & ab & b
    \end{bmatrix}$ and $\mathbf{D}:=\begin{bmatrix}
        1 & 0 & \cdots & 0\\
        a & 1 & \ddots & \vdots\\
        \vdots & \ddots & \ddots & \vdots\\
        a^{n-1} & \cdots & a & 1
    \end{bmatrix}$\\
    $\mathbf{y}=\mathbf{C}\mathbf{u}+\mathbf{D}\mathbf{v}$\\
    Matrices $\mathbf{C}$ and $\mathbf{D}$ are diagonal matrices, so their determinants are the products of their diagonals. 
    Their determinants are non-zero, so they are nonsingular.
    Let $\mathbf{b}={\mathbf{D}}^{-1}\mathbf{y}$ and $\mathbf{A}={\mathbf{D}}^{-1}\mathbf{C}$. 
    $\mathbf{C}=b\mathbf{D}$, so $\mathbf{A}=b\mathbf{I}_n$.
    Thus, the linear least square estimate of $\mathbf{u}^*=\frac{1}{b}\mathbf{D}^{-1}\mathbf{y}=\frac{1}{b}\begin{bmatrix}
        1 & 0 & \cdots & 0\\
        -a & 1 & \ddots & \vdots\\
        \vdots & \ddots & \ddots & \vdots\\
        0 & \cdots & -a & 1
    \end{bmatrix}\mathbf{y}$
    (using row reduction to solve for $\mathbf{D}^{-1}$)
    \item [\textbf{12.10}] \begin{enumerate}
        \item Using $\arcsin(y_i)=\arcsin(\sin(\omega t_i+\theta))=\omega t_i+\theta$ for $-\frac{\pi}{2}\le\omega t_i+\theta\le\frac{\pi}{2}$, we obtain the following system of equations:\\
        $\begin{array}{c}
            \arcsin(y_1)=\omega t_1+\theta\\
            \arcsin(y_2)=\omega t_2+\theta\\
             \vdots\\
            \arcsin(y_p)=\omega t_p+\theta
        \end{array}$
        \item Let $\mathbf{A}:=\begin{bmatrix}
            t_1 & 1\\
            t_2 & 1\\
            \vdots & \vdots\\
            t_p & 1
        \end{bmatrix}$, $\mathbf{x}:=\begin{bmatrix}
            \omega\\
            \theta
        \end{bmatrix}$, and $\mathbf{b}:=\begin{bmatrix}
            \arcsin(y_1)\\
            \arcsin(y_2)\\
            \vdots\\
            \arcsin(y_p)
        \end{bmatrix}$\\
        It follows $\mathbf{x}^*={(\mathbf{A}^\top\mathbf{A})}^{-1}\mathbf{A}^\top\mathbf{b}={\begin{bmatrix}
            p\overline{T^2} & p\overline{T}\\
            p\overline{T} & p
        \end{bmatrix}}^{-1}\begin{bmatrix}
            p\overline{TY}\\
            p\overline{Y}
        \end{bmatrix}$\\
        $={\begin{bmatrix}
            \overline{T^2} & \overline{T}\\
            \overline{T} & 1
        \end{bmatrix}}^{-1}\begin{bmatrix}
            \overline{TY}\\
            \overline{Y}
        \end{bmatrix}=\frac{1}{\overline{T^2}-\overline{T}^2}\begin{bmatrix}
            1 & -\overline{T}\\
            -\overline{T} & \overline{T^2}
        \end{bmatrix}\begin{bmatrix}
            \overline{TY}\\
            \overline{Y}
        \end{bmatrix}$\\
        $=\frac{1}{\overline{T^2}-\overline{T}^2}\begin{bmatrix}
            \overline{TY}-(\overline{T})(\overline{Y})\\
            (\overline{T^2})(\overline{Y})-(\overline{TY})(\overline{T})
        \end{bmatrix}$
    \end{enumerate}
    \item [\textbf{12.11}] Let $\mathbf{A}=\begin{bmatrix}
        1\\
        m
    \end{bmatrix}$ and $\mathbf{b}=\begin{bmatrix}
        x_0\\
        y_0
    \end{bmatrix}$ giving us the least squares minimization problem $\underset{\mathbf{x}}{\argmin}{\lVert \mathbf{Ax}-\mathbf{b}\rVert}^2$.
    Let $\mathbf{x}^*={(\mathbf{A}^\top\mathbf{A})}^{-1}\mathbf{A}^\top\mathbf{b}=\frac{x_0+my_0}{1+m^2}$, so the point closest to $\mathbf{b}$ is
    $\begin{bmatrix}
        \frac{x_0+my_0}{1+m^2}\\
        \frac{mx_0+m^2y_0}{1+m^2}
    \end{bmatrix}$
    \item [\textbf{12.12}] \begin{enumerate}
        \item Let $\mathbf{A}:=\begin{bmatrix}
            \mathbf{x}_1^\top & 1\\
            \mathbf{x}_2^\top & 1\\
            \vdots & \vdots\\
            \mathbf{x}_p^\top & 1\\
        \end{bmatrix}\in \mathbb{R}^{p\times (n+1)}$, $\mathbf{z}:=\begin{bmatrix}
            \mathbf{a}\\
            c
        \end{bmatrix}\in \mathbb{R}^{n+1}$, and $\mathbf{b}:=\begin{bmatrix}
            y_1\\
            y_2\\
            \vdots\\
            y_p
        \end{bmatrix}\in \mathbb{R}^p$.\\
        This gives us the minimization problem $\underset{\mathbf{z}}{\argmin}{\lVert\mathbf{A}\mathbf{z}-\mathbf{b}\rVert}^2$.
        \item Let $\mathbf{X}:=[\mathbf{x}_1,\mathbf{x}_2,\ldots,\mathbf{x}_p]\in \mathbb{R}^{p\times n}$ and $\mathbf{c}={[1,1,\ldots, 1]}^\top\in\mathbb{R}^{p\times 1}$.
        It follows $\mathbf{A}=[\mathbf{X}\thinspace\mathbf{c}]$.
        Thus, $\mathbf{z}^*={(\mathbf{A}^\top\mathbf{A})}^{-1}\mathbf{A}^\top\mathbf{b}$.
        Given $\displaystyle\sum_{i=1}^{p}\mathbf{x}_i=0$,\\ 
        ${(\mathbf{A}^\top\mathbf{A})}^{-1}={\begin{bmatrix}
            \mathbf{X}^\top\mathbf{X} & \mathbf{X}^\top\mathbf{c}\\
            \mathbf{c}^\top\mathbf{X} & \mathbf{c}^\top\mathbf{c}
        \end{bmatrix}}^{-1}={\begin{bmatrix}
            \mathbf{X}^\top\mathbf{X} & 0\\
            0 & p
        \end{bmatrix}}^{-1}=\begin{bmatrix}
            {(\mathbf{X}^\top\mathbf{X})}^{-1} & 0\\
            0 & \frac{1}{p}
        \end{bmatrix}\in\mathbb{R}^{(p+1)\times(p+1)}$.\\
        Given $\displaystyle\sum_{i=1}^{p}\mathbf{y}_i\mathbf{x}_i=0$,\\
        $\mathbf{A}^\top\mathbf{b}=\begin{bmatrix}
            \mathbf{X}^\top\mathbf{b}\\
            \mathbf{c}^\top\mathbf{b}
        \end{bmatrix}=\begin{bmatrix}
            0\\
            \mathbf{c}^\top\mathbf{b}
        \end{bmatrix}\in\mathbb{R}^{p+1}$.\\
        Thus, $\mathbf{z}^*=\begin{bmatrix}
            {(\mathbf{X}^\top\mathbf{X})}^{-1} & 0\\
            0 & \frac{1}{p}
        \end{bmatrix}\begin{bmatrix}
            0\\
            \mathbf{c}^\top\mathbf{b}
        \end{bmatrix}\in\mathbb{R}^{p+1}=\begin{bmatrix}
            0\\
            \frac{1}{p}\mathbf{c}^\top\mathbf{b}
        \end{bmatrix}\in\mathbb{R}^{p+1}$.\\
        Thus, the constant function $\displaystyle f(\mathbf{x})=\frac{1}{p}\sum_{i=1}^{p}y_i$ is the affine function of best fit.
    \end{enumerate}
    \item [\textbf{12.13}] \begin{enumerate}
        \item Let $\mathbf{A}={[u_1,u_2\ldots,u_n]}^\top$ and $\mathbf{b}={[y_1,y_2,\ldots,y_n]}^\top$.\\
        Thus, $\hat{\theta_n}={(\mathbf{A}^\top\mathbf{A})}^{-1}\mathbf{A}^\top\mathbf{b}=\frac{\sum_{k=1}^{n}u_k y_k}{\sum_{k=1}^{n}u_k^2}$ using the least squares approach.
        \item If $u_k=1$ for all $k>0$,
        $\hat{\theta_n}=\displaystyle\lim_{n\rightarrow\infty}\frac{\sum_{k=1}^{n}u_k y_k}{\sum_{k=1}^{n}u_k^2}
        =\lim_{n\rightarrow\infty}\frac{\sum_{k=1}^{n}(\theta+e_k)}{\sum_{k=1}^{n}1}\\
        =\lim_{n\rightarrow\infty}\frac{\theta n+\sum_{k=1}^{n}e_k}{n}\\
        =\theta+\lim_{n\rightarrow\infty}\frac{1}{n}\sum_{k=1}^{n}e_k=\theta\Leftrightarrow\lim_{n\rightarrow\infty}\frac{1}{n}\sum_{k=1}^{n}e_k=0$
    \end{enumerate}
    \item [\textbf{12.14}] Let $\mathbf{A}=\begin{bmatrix}
        0 & 1\\
        1 & 1\\
        2 & 1
    \end{bmatrix}$, $\mathbf{x}=\begin{bmatrix}
        a\\
        b
    \end{bmatrix}$, and $\mathbf{b}=\begin{bmatrix}
        1\\
        2\\
        8
    \end{bmatrix}$.\\
    Thus, $\mathbf{x}^*={(\mathbf{A}^\top\mathbf{A})}^{-1}\mathbf{A}^\top\mathbf{b}=\begin{bmatrix}
        5 & 3\\
        3 & 3
    \end{bmatrix}^{-1}
    \begin{bmatrix}
        18\\
        11
    \end{bmatrix}=\frac{1}{6}\begin{bmatrix}
        3 & -3\\
        -3 & 5
    \end{bmatrix}
    \begin{bmatrix}
        18\\
        11
    \end{bmatrix}=\begin{bmatrix}
        \frac{7}{2}\\
        \frac{1}{6}
    \end{bmatrix}$
    gives us the least squares estimate.
    \item [\textbf{12.22}] ${\lVert\mathbf{Ax}-\mathbf{b}_i\rVert}^2=\mathbf{x}^\top\mathbf{A}^\top\mathbf{A}\mathbf{x}-2\mathbf{x}^\top\mathbf{A}\mathbf{b}_i+{\lVert\mathbf{b}_i\rVert}^2$.\\
    Thus, $\displaystyle\sum_{i=1}^{p}\alpha_i{\lVert\mathbf{Ax}-\mathbf{b}_i\rVert}^2\\
    =(\alpha_1+\alpha_2+\cdots+\alpha_p)\mathbf{x}^\top\mathbf{A}^\top\mathbf{A}\mathbf{x}-2\sum_{i=1}^{p}\alpha_i\mathbf{x}^\top\mathbf{A}\mathbf{b}_i+\sum_{i=1}^{p}\alpha_i{\lVert\mathbf{b}_i\rVert}^2$\\
    which is minimized when\\
    $\displaystyle\mathbf{x}^*={((\alpha_1+\alpha_2+\cdots+\alpha_p)\mathbf{A}^\top\mathbf{A})}^{-1}\mathbf{A}^\top(\alpha_1\mathbf{b}_1+\alpha_2\mathbf{b}_2+\cdots+\alpha_p\mathbf{b}_p)\\
    =\frac{1}{\alpha_1+\alpha_2+\cdots+\alpha_p}\sum_{i=1}^{p}\alpha_i{(\mathbf{A}^\top\mathbf{A})}^{-1}\mathbf{A}^\top\mathbf{b}_i\\
    =\frac{1}{\alpha_1+\alpha_2+\cdots+\alpha_p}\sum_{i=1}^{p}\alpha_i\mathbf{x}_i^*$
    \item [\textbf{12.24}] \begin{enumerate}
        \item \begin{align*}
            &\mathbf{x}^{(0)}={(\mathbf{A}_0^\top\mathbf{A}_0)}^{-1}\mathbf{A}_0^\top\mathbf{b}^{(0)}=\mathbf{G}_0^{-1}\mathbf{A}_0^\top\mathbf{b}^{(0)}\\
            &\mathbf{x}^{(1)}={(\mathbf{A}_1^\top\mathbf{A}_1)}^{-1}\mathbf{A}_1^\top\mathbf{b}^{(1)}=\mathbf{G}_1^{-1}\mathbf{A}_1^\top\mathbf{b}^{(1)}
        \end{align*}
        \item $\mathbf{G}_0=\begin{bmatrix}
            \mathbf{A}_1^\top & \mathbf{a}_1
        \end{bmatrix}\begin{bmatrix}
            \mathbf{A}_1\\
            \mathbf{a}_1^\top
        \end{bmatrix}=\mathbf{A}_1^\top\mathbf{A}_1+\mathbf{a}_1\mathbf{a}_1^\top=\mathbf{G}_1+\mathbf{a}_1\mathbf{a}_1^\top$\\
        Thus, $\mathbf{G}_1=\mathbf{G}_0-\mathbf{a}_1\mathbf{a}_1^\top$\\
        \item $\mathbf{P}_1={(\mathbf{G}_1)}^{-1}\\
        ={(\mathbf{G}_0-\mathbf{a}_1\mathbf{a}_1^\top)}^{-1}\\
        =\mathbf{G}_0^{-1}+\frac{(\mathbf{G}_0^{-1}\mathbf{a}_1)(\mathbf{a}_1^\top\mathbf{G}_0^{-1})}{1-\mathbf{a}_1^\top\mathbf{G}_0^{-1}\mathbf{a}_1}\\
        =\mathbf{P}_0+\frac{\mathbf{P}_0\mathbf{a}_1\mathbf{a}_1^\top\mathbf{P}_0}{1-\mathbf{a}_1^\top\mathbf{P}_0\mathbf{a}_1}$
        \item $\mathbf{A}^\top_0\mathbf{b}^{(0)}=\mathbf{G}_0\mathbf{G}_0^{-1}\mathbf{A}^\top_0\mathbf{b}^{(0)}\\
        =\mathbf{G}_0\mathbf{x}^{(0)}\\
        =(\mathbf{G}_1+\mathbf{a}_1\mathbf{a}_1^\top)\mathbf{x}^{(0)}\\
        =\mathbf{G}_1\mathbf{x}^{(0)}+\mathbf{a}_1\mathbf{a}_1^\top\mathbf{x}^{(0)}$
        \item \begin{align*}
            &\mathbf{x}^{(1)}=\mathbf{G}_1^{-1}\mathbf{A}_1^\top\mathbf{b}^{(1)}\\
            &=\mathbf{G}_1^{-1}\mathbf{A}_1^\top\mathbf{b}^{(1)}\\
            &=\mathbf{G}_1^{-1}(\mathbf{A}_1^\top\mathbf{b}^{(1)}+\mathbf{a}_1b_1-\mathbf{a}_1b_1)\\
            &=\mathbf{G}_1^{-1}(\mathbf{A}_0^\top\mathbf{b}^{(0)}-\mathbf{a}_1b_1)\\
            &=\mathbf{G}_1^{-1}(\mathbf{G}_1\mathbf{x}^{(0)}+\mathbf{a}_1\mathbf{a}_1^\top\mathbf{x}^{(0)}-\mathbf{a}_1b_1)\\
            &=\mathbf{x}^{(0)}+\mathbf{G}_1^{-1}\mathbf{a}_1\mathbf{a}_1^\top\mathbf{x}^{(0)}-\mathbf{G}_1^{-1}\mathbf{a}_1b_1\\
            &=\mathbf{x}^{(0)}-\mathbf{P}_1\mathbf{a}_1(b_1-\mathbf{a}_1^\top\mathbf{x}^{(0)})
        \end{align*}\\
        Thus, \begin{align*}
            &\mathbf{P}_{k+1}=\mathbf{P}_k+\frac{\mathbf{P}_k\mathbf{a}_{k+1}\mathbf{a}_{k+1}^\top\mathbf{P}_k}{1-\mathbf{a}_{k+1}^\top\mathbf{P}_k\mathbf{a}_{k+1}}\\
            &\mathbf{x}^{(k+1)}=\mathbf{x}^{(k)}-\mathbf{P}_{k+1}\mathbf{a}_{k+1}(b_{k+1}-\mathbf{a}_{k+1}^\top\mathbf{x}^{(k)})
        \end{align*}
        gives our update formula
    \end{enumerate}
\end{enumerate}
\end{document}